Engine: remove the measure in the PikeTree-PikeVM(Seen) equivalence proof

Engine/PikeEquiv.v
@@ -17,24 +17,23 @@ Section PikeEquiv.
 (* a tree and a thread are equivalent when they are about to execute the same thing *)
 (* this means when the tree represents a given list of actions, *)
 (* the thread is at a pc that will execute the nfa of that same list of actions *)
-(* the nat is a measure of stuttering steps in the continuation *)
-Inductive tree_thread (code:code) (inp:input) : (tree * group_map) -> thread -> nat -> Prop :=
+Inductive tree_thread (code:code) (inp:input) : (tree * group_map) -> thread -> Prop :=
 | tt_eq:
-  forall tree gm pc b actions n
+  forall tree gm pc b actions
     (TREE: bool_tree rer actions inp b tree)
-    (CONT: actions_rep actions code pc n)
+    (CONT: actions_rep actions code pc)
     (SUBSET: pike_actions actions),
-    tree_thread code inp (tree, gm) (pc, gm, b) n
+    tree_thread code inp (tree, gm) (pc, gm, b)
 | tt_reset:
-  forall tree gm pc b n gidl
-    (TT: tree_thread code inp (tree,GroupMap.reset gidl gm) (pc+1,GroupMap.reset gidl gm,b) n)
+  forall tree gm pc b gidl
+    (TT: tree_thread code inp (tree,GroupMap.reset gidl gm) (pc+1,GroupMap.reset gidl gm,b))
     (RESET: get_pc code pc = Some (ResetRegs gidl)),
-    tree_thread code inp (GroupAction (Reset gidl) tree,gm) (pc,gm,b) n
+    tree_thread code inp (GroupAction (Reset gidl) tree,gm) (pc,gm,b)
 | tt_begin:
-  forall tree gm pc b n
-    (TT: tree_thread code inp (tree,gm) (pc+1,gm,CannotExit) n)
+  forall tree gm pc b
+    (TT: tree_thread code inp (tree,gm) (pc+1,gm,CannotExit))
     (BEGIN: get_pc code pc = Some BeginLoop),
-    tree_thread code inp (tree,gm) (pc,gm,b) (S n).
+    tree_thread code inp (tree,gm) (pc,gm,b).
     
 
 (* the initial active thread and the initial active tree are related with the invariant *)
@@ -43,7 +42,7 @@ Lemma initial_tree_thread:
     (COMPILE: compilation r = code)
     (TREE: bool_tree rer [Areg r] inp CanExit tree)
     (SUBSET: pike_regex r),
-    tree_thread code inp (tree, GroupMap.empty) (0, GroupMap.empty, CanExit) 0.
+    tree_thread code inp (tree, GroupMap.empty) (0, GroupMap.empty, CanExit).
 Proof.
   intros r code tree inp COMPILE TREE SUBSET.
   unfold compilation in COMPILE. destruct (compile r 0) as [c fresh] eqn:COMP.
@@ -57,42 +56,39 @@ Proof.
 Qed.
 
 (* lifting the equivalence predicate to lists *)
-(* the list of nat is the measure, contains the number of stuttering steps for each thread *)
-Inductive list_tree_thread (code:code) (inp:input) : list (tree * group_map) -> list thread -> list nat -> Prop :=
-| ltt_nil: list_tree_thread code inp [] [] []
+Inductive list_tree_thread (code:code) (inp:input) : list (tree * group_map) -> list thread -> Prop :=
+| ltt_nil: list_tree_thread code inp [] []
 | ltt_cons:
-  forall treelist threadlist tree gm pc b measurelist n
-    (LTT: list_tree_thread code inp treelist threadlist measurelist)
-    (TT: tree_thread code inp (tree, gm) (pc, gm, b) n),
-    list_tree_thread code inp ((tree,gm)::treelist) ((pc,gm,b)::threadlist) (n::measurelist).
+  forall treelist threadlist tree gm pc b
+    (LTT: list_tree_thread code inp treelist threadlist)
+    (TT: tree_thread code inp (tree, gm) (pc, gm, b)),
+    list_tree_thread code inp ((tree,gm)::treelist) ((pc,gm,b)::threadlist).
 
 Lemma ltt_app:
-  forall code inp tl1 tl2 vl1 vl2 ml1 ml2
-    (LTT1: list_tree_thread code inp tl1 vl1 ml1)
-    (LTT2: list_tree_thread code inp tl2 vl2 ml2),
-    list_tree_thread code inp (tl1 ++ tl2) (vl1 ++ vl2) (ml1 ++ ml2).
+  forall code inp tl1 tl2 vl1 vl2
+    (LTT1: list_tree_thread code inp tl1 vl1)
+    (LTT2: list_tree_thread code inp tl2 vl2),
+    list_tree_thread code inp (tl1 ++ tl2) (vl1 ++ vl2).
 Proof.
   intros. induction LTT1; auto. simpl. econstructor; eauto.
 Qed.
 
 
 (* lifting the equivalence predicate to pike states, to get the full invariant *)
-Inductive pike_inv (code:code): pike_tree_state -> pike_vm_state -> nat -> Prop :=
+Inductive pike_inv (code:code): pike_tree_state -> pike_vm_state -> Prop :=
 | pikeinv:
-  forall inp treeactive treeblocked threadactive threadblocked best measureactive measureblocked n
-    (ACTIVE: list_tree_thread code inp treeactive threadactive measureactive)
+  forall inp treeactive treeblocked threadactive threadblocked best
+    (ACTIVE: list_tree_thread code inp treeactive threadactive)
     (* blocked threads should be equivalent for the next input *)
     (* nothing to say if there is no next input *)
-    (BLOCKED: forall nextinp, advance_input inp forward = Some nextinp -> list_tree_thread code nextinp treeblocked threadblocked measureblocked)
+    (BLOCKED: forall nextinp, advance_input inp forward = Some nextinp -> list_tree_thread code nextinp treeblocked threadblocked)
     (* these two properties are needed to ensure the two algorithms stop at he same time *)
     (ENDVM: advance_input inp forward = None -> threadblocked = [])
-    (ENDTREE: advance_input inp forward = None -> treeblocked = [])
-    (* the measure is simply the measure of the top priority thread *)
-    (MEASURE: n = hd 0 (measureactive++measureblocked)),
-    pike_inv code (PTS inp treeactive best treeblocked) (PVS inp threadactive best threadblocked) n
+    (ENDTREE: advance_input inp forward = None -> treeblocked = []),
+    pike_inv code (PTS inp treeactive best treeblocked) (PVS inp threadactive best threadblocked)
 | pikeinv_final:
   forall best,
-    pike_inv code (PTS_final best) (PVS_final best) 0.
+    pike_inv code (PTS_final best) (PVS_final best).
 
 (** * Invariant Initialization  *)
 
@@ -102,9 +98,9 @@ Lemma initial_pike_inv:
     (TREE: bool_tree rer [Areg r] inp CanExit tree)
     (COMPILE: compilation r = code)
     (SUBSET: pike_regex r),
-    pike_inv code (pike_tree_initial_state tree inp) (pike_vm_initial_state inp) 0.
+    pike_inv code (pike_tree_initial_state tree inp) (pike_vm_initial_state inp).
 Proof.
-  intros r inp tree code TREE COMPILE SUBSET.         
+  intros r inp tree code TREE COMPILE SUBSET.
   unfold compilation in COMPILE. destruct (compile r 0) as [c fresh] eqn:COMP.
   apply compile_nfa_rep with (prev := []) in COMP as REP; auto. simpl in REP.
   apply fresh_correct in COMP. simpl in COMP. subst.
@@ -180,10 +176,10 @@ Ltac stutter :=
 
 Ltac invert_rep :=
    match goal with
-   | [ H : actions_rep (Areg _ :: _) _ _ _ |- _ ] => inversion H; clear H; subst; try no_stutter
-   | [ H : actions_rep (Aclose _ :: _) _ _ _ |- _ ] => inversion H; clear H; subst; try no_stutter
-   | [ H : actions_rep (Acheck _ :: _) _ _ _ |- _ ] => inversion H; clear H; subst; try no_stutter
-   | [ H : actions_rep [] _ _ _ |- _ ] => inversion H; clear H; subst; try no_stutter
+   | [ H : actions_rep (Areg _ :: _) _ _ |- _ ] => inversion H; clear H; subst; try no_stutter
+   | [ H : actions_rep (Aclose _ :: _) _ _ |- _ ] => inversion H; clear H; subst; try no_stutter
+   | [ H : actions_rep (Acheck _ :: _) _ _ |- _ ] => inversion H; clear H; subst; try no_stutter
+   | [ H : actions_rep [] _ _ |- _ ] => inversion H; clear H; subst; try no_stutter
    | [ H : action_rep (Areg _) _ _ _ |- _ ] => inversion H; clear H; subst; try no_stutter
    | [ H : action_rep (Aclose _) _ _ _ |- _ ] => inversion H; clear H; subst; try no_stutter
    | [ H : action_rep (Acheck _) _ _ _ |- _ ] => inversion H; clear H; subst; try no_stutter
@@ -207,13 +203,13 @@ Section PikeEquiv2.
 (* These lemmas discard the stuttering steps by preventing the current pc being at a Jmp instruction *)
 
 Theorem generate_match:
-  forall tree gm inp code pc b n
+  forall tree gm inp code pc b
     (TREESTEP: tree_bfs_step tree gm (idx inp) = StepMatch)
     (NOSTUTTER: stutters pc code = false)
-    (TT: tree_thread rer code inp (tree, gm) (pc, gm, b) n),
+    (TT: tree_thread rer code inp (tree, gm) (pc, gm, b)),
     epsilon_step rer (pc, gm, b) code inp = EpsMatch.
 Proof.
-  intros tree gm inp code pc b n TREESTEP NOSTUTTER TT.
+  intros tree gm inp code pc b TREESTEP NOSTUTTER TT.
   unfold tree_bfs_step in TREESTEP. destruct tree; inversion TREESTEP. subst. clear TREESTEP.
   inversion TT; subst; try no_stutter.
   remember Match as TMATCH.
@@ -231,15 +227,15 @@ Proof.
 
 
 Theorem generate_blocked:
-  forall tree gm inp code pc b nexttree n
+  forall tree gm inp code pc b nexttree
     (TREESTEP: tree_bfs_step tree gm (idx inp) = StepBlocked nexttree)
     (NOSTUTTER: stutters pc code = false)
-    (TT: tree_thread rer code inp (tree, gm) (pc, gm, b) n),
+    (TT: tree_thread rer code inp (tree, gm) (pc, gm, b)),
     epsilon_step rer (pc,gm,b) code inp = EpsBlocked (pc+1,gm,CanExit) /\
-      (forall nextinp, advance_input inp forward = Some nextinp -> tree_thread rer code nextinp (nexttree,gm) (pc+1,gm,CanExit) n) /\
+      (forall nextinp, advance_input inp forward = Some nextinp -> tree_thread rer code nextinp (nexttree,gm) (pc+1,gm,CanExit)) /\
       exists nextinp, advance_input inp forward = Some nextinp.
 Proof.
-  intros tree gm inp code pc b nexttree n TREESTEP NOSTUTTER TT.
+  intros tree gm inp code pc b nexttree TREESTEP NOSTUTTER TT.
   unfold tree_bfs_step in TREESTEP. destruct tree; inversion TREESTEP. subst. clear TREESTEP.
   inversion TT; subst; try no_stutter.
   remember (Read c nexttree) as TREAD.
@@ -261,13 +257,13 @@ Qed.
 
 
 Theorem generate_open:
-  forall gid tree gm inp code pc b n
-    (TT: tree_thread rer code inp (GroupAction (Open gid) tree, gm) (pc, gm, b) n)
+  forall gid tree gm inp code pc b
+    (TT: tree_thread rer code inp (GroupAction (Open gid) tree, gm) (pc, gm, b))
     (NOSTUTTER: stutters pc code = false),
     epsilon_step rer (pc, gm, b) code inp = EpsActive [(pc + 1, GroupMap.open (idx inp) gid gm, b)] /\
-      tree_thread rer code inp (tree,GroupMap.open (idx inp) gid gm) (pc + 1, GroupMap.open (idx inp) gid gm, b) n.
+      tree_thread rer code inp (tree,GroupMap.open (idx inp) gid gm) (pc + 1, GroupMap.open (idx inp) gid gm, b).
 Proof.
-  intros gid tree gm inp code pc b n TT NOSTUTTER.
+  intros gid tree gm inp code pc b TT NOSTUTTER.
   inversion TT; subst; try invert_rep.
   remember (GroupAction (Open gid) tree) as TOPEN.
   induction TREE; intros; subst; try inversion HeqTOPEN; subst.
@@ -286,18 +282,19 @@ Qed.
 
 
 Theorem generate_close:
-  forall gid tree gm inp code pc b n
-    (TT: tree_thread rer code inp (GroupAction (Close gid) tree, gm) (pc, gm, b) n)
+  forall gid tree gm inp code pc b
+    (TT: tree_thread rer code inp (GroupAction (Close gid) tree, gm) (pc, gm, b))
     (NOSTUTTER: stutters pc code = false),
     epsilon_step rer (pc, gm, b) code inp = EpsActive [(pc + 1, GroupMap.close (idx inp) gid gm, b)] /\
-      tree_thread rer code inp (tree,GroupMap.close (idx inp) gid gm) (pc + 1, GroupMap.close (idx inp) gid gm, b) n.
+      tree_thread rer code inp (tree,GroupMap.close (idx inp) gid gm) (pc + 1, GroupMap.close (idx inp) gid gm, b).
 Proof.
-  intros gid tree gm inp code pc b n TT NOSTUTTER.
+  intros gid tree gm inp code pc b TT NOSTUTTER.
   inversion TT; subst; try no_stutter.
   remember (GroupAction (Close gid) tree) as TCLOSE.
   induction TREE; intros; subst; try inversion HeqTCLOSE; subst.
-  - repeat invert_rep. simpl. rewrite CLOSE. pike_subset.
-    econstructor; eauto. replace (pc + 1) with (S pc) by lia. eauto.
+  - repeat invert_rep. simpl. rewrite CLOSE. split; auto.
+    econstructor; eauto. 2: pike_subset.
+    replace (pc + 1) with (S pc) by lia. auto. 
   - repeat invert_rep. eapply IHTREE; eauto. pike_subset.
   - repeat invert_rep. eapply IHTREE; eauto. pike_subset.
     repeat (econstructor; eauto). pike_subset.
@@ -323,11 +320,11 @@ Proof.
 Qed.
 
 Corollary generate_reset:  
-  forall gidl tree inp code pc b gm n
-    (TT: tree_thread rer code inp (GroupAction (Reset gidl) tree, gm) (pc,gm,b) n)
+  forall gidl tree inp code pc b gm
+    (TT: tree_thread rer code inp (GroupAction (Reset gidl) tree, gm) (pc,gm,b))
     (NOSTUTTER: stutters pc code = false),
     epsilon_step rer (pc,gm,b) code inp = EpsActive [(pc+1, GroupMap.reset gidl gm, b)] /\
-      tree_thread rer code inp (tree,GroupMap.reset gidl gm) (pc+1, GroupMap.reset gidl gm, b) n.
+      tree_thread rer code inp (tree,GroupMap.reset gidl gm) (pc+1, GroupMap.reset gidl gm, b).
 Proof.
   intros.
   inversion TT; subst.
@@ -337,12 +334,12 @@ Proof.
 Qed.
 
 Theorem generate_mismatch:
-  forall gm inp code pc b n
-    (TT: tree_thread rer code inp (Mismatch, gm) (pc, gm, b) n)
+  forall gm inp code pc b
+    (TT: tree_thread rer code inp (Mismatch, gm) (pc, gm, b))
     (NOSTUTTER: stutters pc code = false),
     epsilon_step rer (pc, gm, b) code inp = EpsActive [].
 Proof.
-  intros gm inp code pc b n TT NOSTUTTER.
+  intros gm inp code pc b TT NOSTUTTER.
   inversion TT; subst; try no_stutter.
   remember (Mismatch) as TMIS.
   induction TREE; intros; subst; try inversion HeqTMIS; subst.
@@ -358,13 +355,13 @@ Proof.
 Qed.
 
 Theorem generate_checkpass:
-  forall tree gm inp code pc b n
-    (TT: tree_thread rer code inp (Progress tree, gm) (pc, gm, b) n)
+  forall tree gm inp code pc b
+    (TT: tree_thread rer code inp (Progress tree, gm) (pc, gm, b))
     (NOSTUTTER: stutters pc code = false),
     exists nextpc, epsilon_step rer (pc, gm, b) code inp = EpsActive [(nextpc,gm,CanExit)] /\
-      tree_thread rer code inp (tree,gm) (nextpc,gm,CanExit) n.
+      tree_thread rer code inp (tree,gm) (nextpc,gm,CanExit).
 Proof.
-  intros tree gm inp code pc b n TT NOSTUTTER.
+  intros tree gm inp code pc b TT NOSTUTTER.
   inversion TT; subst; try no_stutter.
   remember (Progress tree) as TPASS.
   induction TREE; intros; subst; try inversion HeqTPASS; subst.
@@ -379,22 +376,21 @@ Qed.
 
 
 Theorem generate_choice:
-  forall tree1 tree2 gm inp code pc b treeactive n
+  forall tree1 tree2 gm inp code pc b treeactive
     (TREESTEP: tree_bfs_step (Choice tree1 tree2) gm (idx inp) = StepActive treeactive)
     (NOSTUTTER: stutters pc code = false)
-    (TT: tree_thread rer code inp (Choice tree1 tree2, gm) (pc, gm, b) n),
-  exists threadactive measure,
+    (TT: tree_thread rer code inp (Choice tree1 tree2, gm) (pc, gm, b)),
+  exists threadactive,
     epsilon_step rer (pc, gm, b) code inp = EpsActive threadactive /\
-      list_tree_thread rer code inp treeactive threadactive measure.
+      list_tree_thread rer code inp treeactive threadactive.
 Proof.
-  intros tree1 tree2 gm inp code pc b treeactive n TREESTEP NOSTUTTER TT.
+  intros tree1 tree2 gm inp code pc b treeactive TREESTEP NOSTUTTER TT.
   unfold tree_bfs_step in TREESTEP. inversion TREESTEP. subst. clear TREESTEP.
   inversion TT; subst; try no_stutter.
   remember (Choice tree1 tree2) as TCHOICE.
   induction TREE; intros; subst; try inversion HeqTCHOICE; subst.
   - repeat invert_rep. eapply IHTREE; eauto. pike_subset.
-  - repeat invert_rep. exists [(S pc,gm,b);(S end1,gm,b)]. exists [S n; n]. split.
-  (* here in the first element of the list we introduced an extra stuttering step, hence the (S n) measure *)
+  - repeat invert_rep. exists [(S pc,gm,b);(S end1,gm,b)]. split.
     + unfold epsilon_step. rewrite FORK. auto.
     + constructor.
       * constructor. constructor.
@@ -412,7 +408,7 @@ Proof.
   - (* when the choice comes from a star *)
     repeat invert_rep. destruct greedy; inversion CHOICE; subst; destruct plus; inversion H1.
     +                           (* greedy star *)
-      simpl. rewrite FORK. exists [(S pc, gm, b); (S end1, gm, b)]. exists [S n; n]. split; auto.
+      simpl. rewrite FORK. exists [(S pc, gm, b); (S end1, gm, b)]. split; auto.
       econstructor.
       * econstructor. constructor.
         apply tt_eq with (actions:=cont); auto. pike_subset.
@@ -426,7 +422,7 @@ Proof.
         repeat (econstructor; eauto).
         replace (S (S pc)) with (S pc + 1) by lia. auto.
     +                           (* lazy star *)
-      simpl. rewrite FORK. exists [(S end1, gm, b); (S pc, gm, b)]. exists [n; S n]. split; auto.
+      simpl. rewrite FORK. exists [(S end1, gm, b); (S pc, gm, b)]. split; auto.
       econstructor.
       * constructor. constructor. apply tt_begin; auto.
         replace (S (S pc)) with (S pc + 1) in RESET by lia.
@@ -443,36 +439,36 @@ Qed.
 
 (* next we combine the generate lemmas together, for the general non-stuttering case *)
 Theorem generate_active:
-  forall tree gm inp code pc b treeactive n
+  forall tree gm inp code pc b treeactive
     (TREESTEP: tree_bfs_step tree gm (idx inp) = StepActive treeactive)
     (NOSTUTTER: stutters pc code = false)
-    (TT: tree_thread rer code inp (tree, gm) (pc, gm, b) n),
-  exists threadactive measure,
+    (TT: tree_thread rer code inp (tree, gm) (pc, gm, b)),
+  exists threadactive,
     epsilon_step rer (pc, gm, b) code inp = EpsActive threadactive /\
-      list_tree_thread rer code inp treeactive threadactive measure.
+      list_tree_thread rer code inp treeactive threadactive.
 Proof.
-  intros tree gm inp code pc b treeactive n TREESTEP NOSTUTTER TT.
+  intros tree gm inp code pc b treeactive TREESTEP NOSTUTTER TT.
   destruct tree; simpl in TREESTEP; inversion TREESTEP; subst.
-  - eapply generate_mismatch in TT; auto. exists []. exists []. split; eauto. constructor.
+  - eapply generate_mismatch in TT; auto. exists []. split; eauto. constructor.
   - eapply generate_choice; eauto.
   - inversion TT; subst; try no_stutter.
     eapply subset_semantics in TREE as SUBSETTREE; auto.
     inversion SUBSETTREE.
   - eapply generate_checkpass in TT as [nextpc [STEP EQ]]; auto.
-    exists [(nextpc,gm,CanExit)]. exists [n]. split; eauto.
+    exists [(nextpc,gm,CanExit)]. split; eauto.
     constructor; auto. constructor.
   - inversion TT; subst; try no_stutter.
     eapply subset_semantics in TREE as SUBSETTREE; auto.
     inversion SUBSETTREE.
   - destruct g.
     + eapply generate_open in TT as [STEP EQ]; auto.
-      exists [(pc+1,GroupMap.open (idx inp) g gm,b)]. exists [n]. split; eauto.
+      exists [(pc+1,GroupMap.open (idx inp) g gm,b)]. split; eauto.
       constructor; auto. constructor.
     + eapply generate_close in TT as [STEP EQ]; auto.
-      exists [(pc+1,GroupMap.close (idx inp) g gm,b)]. exists [n]. split; eauto.
+      exists [(pc+1,GroupMap.close (idx inp) g gm,b)]. split; eauto.
       constructor; auto. constructor.
     + eapply generate_reset in TT as [STEP EQ]; auto.
-      exists [(pc + 1, GroupMap.reset gl gm, b)]. exists [n]. split; eauto.
+      exists [(pc + 1, GroupMap.reset gl gm, b)]. split; eauto.
       constructor; auto. constructor.
   - inversion TT; subst; try no_stutter.
     eapply subset_semantics in TREE as SUBSETTREE; auto.
@@ -483,90 +479,89 @@ Proof.
 Qed.
 
 (* TODO: simplify/automate this proof *)
-(* in the case where we are at a stuttering step, we show that we still preserve the invariant and decrease the measure *)
+(* in the case where we are at a stuttering step, we show that we still preserve the invariant *)
 Theorem stutter_step:
-  forall tree gm inp code pc b n
-    (TT: tree_thread rer code inp (tree,gm) (pc,gm,b) n)
+  forall tree gm inp code pc b
+    (TT: tree_thread rer code inp (tree,gm) (pc,gm,b))
     (STUTTER: stutters pc code = true),
-  exists nextpc nextb m,
+  exists nextpc nextb,
     epsilon_step rer (pc,gm,b) code inp = EpsActive [(nextpc,gm,nextb)] /\
-      tree_thread rer code inp (tree,gm) (nextpc,gm,nextb) m /\
-      n = S m.
+      tree_thread rer code inp (tree,gm) (nextpc,gm,nextb).
 Proof.
-  intros tree gm inp code pc b n TT STUTTER.
+  intros tree gm inp code pc b TT STUTTER.
   inversion TT; subst.
   (* reset is not stuttering *)
   2: { unfold stutters in STUTTER. rewrite RESET in STUTTER. inversion STUTTER. }
   (* at a beginloop instruction *)
-  2: { exists (pc + 1). exists CannotExit. exists n0. split; try split; auto.
+  2: { exists (pc + 1). exists CannotExit. split; try split; auto.
        simpl. rewrite BEGIN. auto. }
   (* at a jmp instruction *)
-  generalize dependent pc. generalize dependent n.
+  generalize dependent pc.
   induction TREE; intros.
   - invert_rep. stutter.
-    exists pcstart. exists b. exists n0. split; try split; try lia.
+    exists pcstart. exists b. split; try split; try lia.
     + simpl. rewrite JMP. auto.
-    + apply tt_eq with (actions:=[]); try constructor; auto.
+    + apply tt_eq with (actions:=[]); auto; constructor; auto.
   - invert_rep.
     { invert_rep. stutter. }
-    exists pcstart. exists CanExit. exists n0. split; try split; try lia.
-    + simpl. rewrite JMP. auto.
-    + apply tt_eq with (actions:=Acheck strcheck::cont); try constructor; auto; pike_subset.
-  - invert_rep.
-    { invert_rep. stutter. }
-    exists pcstart. exists CannotExit. exists n0. split; try split; try lia.
+    exists pcstart. exists CanExit. split; try split; try lia.
     + simpl. rewrite JMP. auto.
     + apply tt_eq with (actions:=Acheck strcheck::cont); try constructor; auto; pike_subset.
   - invert_rep.
     { invert_rep. stutter. }
-    exists pcstart. exists b. exists n0. split; try split; try lia.
+    exists pcstart. exists CannotExit. split; try split; try lia.
+    + simpl. rewrite JMP. auto.
+    + apply tt_eq with (actions:=Acheck strcheck::cont); try constructor; auto; pike_subset.
+  - invert_rep.
+    { invert_rep. stutter. }
+    exists pcstart. exists b. split; try split; try lia.
     + simpl. rewrite JMP. auto.
     + apply tt_eq with (actions:=Aclose gid::cont); try constructor; auto; pike_subset.
   - invert_rep.
     + invert_rep. invert_rep; try in_subset.
       eapply IHTREE; eauto. pike_subset.
-    + exists pcstart. exists b. exists n0. split; try split; try lia.
+    + exists pcstart. exists b. split; try split; try lia.
       * simpl. rewrite JMP. auto.
       * apply tt_eq with (actions:=Areg Epsilon :: cont); try constructor; auto; pike_subset.
   - invert_rep.
     { invert_rep. invert_rep; try in_subset; try stutter. }
-    exists pcstart. exists b. exists n0. split; try split; try lia.
+    exists pcstart. exists b. split; try split; try lia.
     + simpl. rewrite JMP. auto.
     + apply tt_eq with (actions:=Areg (Regex.Character cd) :: cont); try constructor; auto; pike_subset.
       eapply tree_char; eauto.
   - invert_rep.
     { invert_rep. invert_rep; try in_subset; try stutter. }
-    exists pcstart. exists b. exists n0. split; try split; try lia.
+    exists pcstart. exists b. split; try split; try lia.
     + simpl. rewrite JMP. auto.
     + apply tt_eq with (actions:=Areg (Regex.Character cd) :: cont); try constructor; auto; pike_subset.
   - invert_rep.
     { invert_rep. invert_rep; try in_subset; try stutter. }
-    exists pcstart. exists b. exists n0. split; try split; try lia.
+    exists pcstart. exists b. split; try split; try lia.
     * simpl. rewrite JMP. auto.
     * apply tt_eq with (actions:=Areg (Disjunction r1 r2) :: cont); try constructor; auto; pike_subset.
   - invert_rep.
     + invert_rep. invert_rep; try in_subset.
       eapply IHTREE; eauto. pike_subset.
       repeat (econstructor; eauto).
-    + exists pcstart. exists b. exists n0. split; try split; try lia.
+    + exists pcstart. exists b. split; try split; try lia.
       * simpl. rewrite JMP. auto.
       * apply tt_eq with (actions:=Areg (Sequence r1 r2) :: cont); try constructor; auto; pike_subset.
   - invert_rep.
     { invert_rep. invert_rep; try in_subset; try stutter. }
-    exists pcstart. exists b. exists n0. split; try split; try lia.
+    exists pcstart. exists b. split; try split; try lia.
     * simpl. rewrite JMP. auto.
     * apply tt_eq with (actions:=Areg (Quantified greedy (S min) plus r1) :: cont); try constructor; auto; pike_subset.
   - pike_subset.
   - invert_rep.
     { invert_rep. invert_rep; try in_subset. destruct greedy; stutter. }
-    exists pcstart. exists b. exists n0. split; try split; try lia.
+    exists pcstart. exists b. split; try split; try lia.
     + simpl. rewrite JMP. auto.
-    + pike_subset. destruct plus; inversion H3. simpl in CONT0.
+    + destruct plus; [pike_subset|].
       apply tt_eq with (actions:=Areg (Quantified greedy 0 (NoI.N 1 + +∞)%NoI r1) :: cont); try constructor; auto; pike_subset.
       eapply tree_quant_free; eauto.
   - invert_rep.
     { invert_rep. invert_rep; try in_subset; try stutter. }
-    exists pcstart. exists b. exists n0. split; try split; try lia.
+    exists pcstart. exists b. split; try split; try lia.
     * simpl. rewrite JMP. auto.
     * apply tt_eq with (actions:=Areg (Group gid r1):: cont); try constructor; auto; pike_subset.
   - pike_subset.
@@ -575,31 +570,30 @@ Qed.
 
 
 Theorem invariant_preservation:
-  forall code pts1 pvs1 n pts2
-    (INV: pike_inv rer code pts1 pvs1 n)
+  forall code pts1 pvs1 pts2
+    (INV: pike_inv rer code pts1 pvs1)
     (TREESTEP: pike_tree_step pts1 pts2),
     (* progress on the PTS side implies progress on the PVS side *)
     (        
-      exists pvs2 m,
+      exists pvs2,
         pike_vm_step rer code pvs1 pvs2 /\
-          pike_inv rer code pts2 pvs2 m
+          pike_inv rer code pts2 pvs2
     )
     \/
       (* stuttering step on the PVS side *)
       (
-        exists pvs2 m,
+        exists pvs2,
           pike_vm_step rer code pvs1 pvs2 /\
-            pike_inv rer code pts1 pvs2 m /\
-            m < n
+            pike_inv rer code pts1 pvs2
       ).
 Proof.
-  intros code pts1 pvs1 n pts2 INV TREESTEP.
+  intros code pts1 pvs1 pts2 INV TREESTEP.
   inversion INV; subst.
   (* Final states make no step *)
   2: { left. intros. inversion TREESTEP. }
   inversion TREESTEP; subst.
   (* pts_final *)
-  - left. exists (PVS_final best). exists 0. split.
+  - left. exists (PVS_final best). split.
     + inversion ACTIVE. subst.
       destruct (advance_input inp) eqn:ADVANCE.
       * specialize (BLOCKED i eq_refl). inversion BLOCKED. subst. apply pvs_final.
@@ -611,46 +605,46 @@ Proof.
     destruct (advance_input inp) as [nextinp|] eqn:ADVANCE.
     + specialize (BLOCKED nextinp eq_refl).
       inversion BLOCKED. subst.
-      exists (PVS nextinp ((pc,gm,b)::threadlist) best []). exists n. split.
+      exists (PVS nextinp ((pc,gm,b)::threadlist) best []). split.
       * apply pvs_nextchar. auto.
       * apply advance_next in ADVANCE. subst. eapply pikeinv; eauto. intros. constructor.
     + specialize (ENDTREE eq_refl). inversion ENDTREE.
   (* pts_active *)
   - inversion ACTIVE. subst.
     destruct (stutters pc code) eqn:STUTTERS.
-    + right. apply stutter_step in TT as [nextpc [nextb [m [EPSSTEP [TT LESS]]]]]; subst; eauto.
-      exists (PVS inp ([(nextpc, gm, nextb)] ++ threadlist) best threadblocked). exists m.
+    + right. apply stutter_step in TT as [nextpc [nextb [EPSSTEP TT]]]; subst; eauto.
+      exists (PVS inp ([(nextpc, gm, nextb)] ++ threadlist) best threadblocked).
       split; try split; auto.
       * apply pvs_active. auto.
-      * simpl. eapply pikeinv with (measureactive:=m::measurelist); eauto. econstructor; eauto.
+      * simpl. eapply pikeinv; eauto. econstructor; eauto.
     + left. inversion ACTIVE. subst. rename t into tree.
-      eapply generate_active in TT as [newthreads [measure [EPS LTT2]]]; eauto.
-      exists (PVS inp (newthreads++threadlist) best threadblocked). exists (hd 0 ((measure ++ measurelist) ++ measureblocked)). split.
+      eapply generate_active in TT as [newthreads [EPS LTT2]]; eauto.
+      exists (PVS inp (newthreads++threadlist) best threadblocked). split.
       * apply pvs_active. auto.
       * eapply pikeinv; auto. apply ltt_app; eauto.
   (* pts_match *)
   - inversion ACTIVE. subst.
      destruct (stutters pc code) eqn:STUTTERS.
-    + right. apply stutter_step in TT as [nextpc [nextb [m [EPSSTEP [TT LESS]]]]]; subst; eauto.
-      exists (PVS inp ([(nextpc, gm, nextb)] ++ threadlist) best threadblocked). exists m.
+    + right. apply stutter_step in TT as [nextpc [nextb [EPSSTEP TT]]]; subst; eauto.
+      exists (PVS inp ([(nextpc, gm, nextb)] ++ threadlist) best threadblocked).
       split; try split; auto.
       * apply pvs_active. auto.
-      * simpl. eapply pikeinv with (measureactive:=m::measurelist); eauto. econstructor; eauto.
+      * simpl. eapply pikeinv; eauto. econstructor; eauto.
     + left. rename t into tree. eapply generate_match in TT; eauto.
-      exists (PVS inp [] (Some (inp,gm)) threadblocked). exists (hd 0 measureblocked). split.
+      exists (PVS inp [] (Some (inp,gm)) threadblocked). split.
       * apply pvs_match. auto.
-      * econstructor; auto. constructor. simpl. auto.
+      * econstructor; auto. constructor.
   (* pts_blocked *)
   - inversion ACTIVE. subst.
     destruct (stutters pc code) eqn:STUTTERS.
-    + right. apply stutter_step in TT as [nextpc [nextb [m [EPSSTEP [TT LESS]]]]]; subst; eauto.
-      exists (PVS inp ([(nextpc, gm, nextb)] ++ threadlist) best threadblocked). exists m.
+    + right. apply stutter_step in TT as [nextpc [nextb [EPSSTEP TT]]]; subst; eauto.
+      exists (PVS inp ([(nextpc, gm, nextb)] ++ threadlist) best threadblocked).
       split; try split; auto.
       * apply pvs_active. auto.
-      * simpl. eapply pikeinv with (measureactive:=m::measurelist); eauto. econstructor; eauto.
+      * simpl. eapply pikeinv; eauto. econstructor; eauto.
     + left. rename t into tree.
-      specialize (generate_blocked _ _ _ _ _ _ _ _ STEP STUTTERS TT) as [EPS2 [TT2 [nexti ADVANCE]]].
-      exists (PVS inp threadlist best (threadblocked ++ [(pc+1,gm,CanExit)])). exists (hd 0 (measurelist ++ measureblocked ++ [n])). split.
+      specialize (generate_blocked _ _ _ _ _ _ _ STEP STUTTERS TT) as [EPS2 [TT2 [nexti ADVANCE]]].
+      exists (PVS inp threadlist best (threadblocked ++ [(pc+1,gm,CanExit)])). split.
       * apply pvs_blocked. auto.
       * econstructor; eauto.
         2: { intros H. rewrite ADVANCE in H. inversion H. }
@@ -659,34 +653,5 @@ Proof.
         apply ltt_app; eauto. specialize (TT2 nextinp H).
         eapply ltt_cons. constructor. auto.
 Qed.
-
-
-(** * Backward Style Invariant Preservation *)
-(* Deprecated *)
-(* Theorem backward_match: *)
-(*   forall tree gm idx inp code pc b n *)
-(*     (VMSTEP: epsilon_step (pc,gm,b) code inp idx = EpsMatch) *)
-(*     (NOSTUTTER: stutters pc code = false) *)
-(*     (TT: tree_thread code inp (tree, gm) (pc, gm, b) n), *)
-(*     tree = Match. *)
-(* Proof. *)
-(*   intros tree gm idx inp code pc b n VMSTEP NOSTUTTER TT. *)
-(*   simpl in VMSTEP. *)
-(*   (* extracting current instruction *) *)
-(*   destruct (get_pc code pc) as [instr|] eqn:CODE. *)
-(*   2: { inversion VMSTEP. } *)
-(*   destruct instr; try solve [inversion VMSTEP]. *)
-(*   2: { destruct (check_read c inp); inversion VMSTEP. } *)
-(*   2: { destruct b; inversion VMSTEP. } *)
-(*   (* extracting relevant invariant case *) *)
-(*   inversion TT; subst. *)
-(*   2: { rewrite RESET in CODE. inversion CODE. } *)
-(*   2: { rewrite BEGIN in CODE. inversion CODE. } *)
-(*   (* there are many ways that we could be at an Accept instruction *) *)
-(*   (* we could have r = epsilon, cont = [] *) *)
-(*   (* or r = Epsilon;Epsilon, cont = []... *) *)
-(* Abort. *)
-(* It's really harder to reason from the VM step *)
-(* It's much easier to reason from a Pike tree step, ast it allows inductive reasoning on the bool_tree semantics  *)
 
 End PikeEquiv2.
